src/BBSmod.v
@@ -8,11 +8,11 @@ Set Implicit Arguments.
 Unset Strict Implicit.
 Import Prenex Implicits.
 
-Definition smodB bs1 bs2 : bits :=
-  let r_sdiv := sremB bs1 bs2 in 
-  if (msb bs1 == msb bs2) || (r_sdiv == (zeros (size r_sdiv))) then
-    r_sdiv
-  else addB r_sdiv bs2.
+(* Definition smodB bs1 bs2 : bits := *)
+(*   let r_sdiv := sremB' bs1 bs2 in  *)
+(*   if (msb bs1 == msb bs2) || (r_sdiv == (zeros (size r_sdiv))) then *)
+(*     r_sdiv *)
+(*   else addB r_sdiv bs2. *)
 
 (* ===== bit_blast_smod ===== *)
 
@@ -33,12 +33,6 @@ Definition bit_blast_smod g ls1 ls2 : generator * cnf * word :=
             let '(g_add2, cs_add2, lrs_add2) := bit_blast_add g_and2 lrs_srem lrs_and2 in
             (g_add2, catrev cs_srem (catrev cs_eq (catrev cs_eq2 (catrev cs_or (catrev cs_not (catrev cs_and2 cs_add2))))), lrs_add2).
 
-Lemma size_sremB : forall bs1 bs2, size (sremB bs1 bs2) = size bs1.
-Proof.
-  intros. rewrite /sremB /absB.
-  case (msb bs1); case (msb bs2); try rewrite size_negB size_uremB size_negB//;
-                                      try rewrite size_uremB//.
-Qed.
 
 Lemma bit_blast_srem_size_ss g ls1 ls2 g' cs lrs_r:
   bit_blast_srem g ls1 ls2 = (g', cs, lrs_r) ->
@@ -58,14 +52,14 @@ Lemma orB0: forall (n : nat) (bs : bits), (bs||# zeros n)%bits = bs.
 Proof. Admitted.
  *)
 
-Lemma bit_blast_smod_correct g ls1 ls2 g' cs rlrs E bs1 bs2 :
+Lemma bit_blast_smod_correct' g ls1 ls2 g' cs rlrs E bs1 bs2 :
   bit_blast_smod g ls1 ls2 = (g', cs, rlrs) ->
   size ls1 = size ls2 ->
   0 < size ls2 ->
   enc_bits E ls1 bs1 ->
   enc_bits E ls2 bs2 ->
   interp_cnf E (add_prelude cs) ->
-  enc_bits E rlrs (smodB bs1 bs2).
+  enc_bits E rlrs (smodB' bs1 bs2).
 Proof.
   rewrite /bit_blast_smod.
   dcase (bit_blast_srem g ls1 ls2) => [[[g_srem] cs_srem] r_rem] Hbbsrem.
@@ -80,7 +74,7 @@ Proof.
   - rewrite/=; case => _ <- <-.
     move => Hsz12 Hgt02 Henc1 Henc2.
     rewrite 2!add_prelude_catrev. move/andP => [Hcssrem Hcsu]; move/andP : Hcsu => [Hcseq2 Hcseq].
-    rewrite/smodB.
+    rewrite/smodB'.
     move : (add_prelude_tt Hcssrem) => Htt. 
     have Hszmsl12 : size [:: (splitmsl ls1).2] = size [:: (splitmsl ls2).2] by done.
     move/andP : (enc_bits_splitmsb Htt Henc1) => [Henc1r Hencmsb1].
@@ -91,20 +85,20 @@ Proof.
     rewrite (eqP Heq). (*in Henceqr. generalize Henceqr.*)
     rewrite (add_prelude_enc_bit_true ([:: (splitmsb bs1).2] == [:: (splitmsb bs2).2]) Hcseq) Seqs.singleton_eq-/(msb bs1) -/(msb bs2).
     move => Hmsb12. rewrite Hmsb12 orTb. 
-    move : (bit_blast_srem_correct Hbbsrem Hsz12 Hgt02 Henc1 Henc2 Hcssrem) => Hencr; done.
+    move : (bit_blast_srem_correct Hbbsrem Hsz12 Hgt02 Henc1 Henc2 Hcssrem) => Hencr. by rewrite -sremB_is_sremB'.
   - rewrite /=; case => _ <- <-. move => Hsz12 Hgt02 Henc1 Henc2.
-    rewrite 2!add_prelude_catrev /smodB. move/andP => [Hcssrem Hcsu]; move/andP : Hcsu => [Hcseq2 Hcseq].
+    rewrite 2!add_prelude_catrev /smodB'. move/andP => [Hcssrem Hcsu]; move/andP : Hcsu => [Hcseq2 Hcseq].
     have Hszcprrem : size r_rem = size (copy (size r_rem) lit_ff) by rewrite size_nseq.
     move : (add_prelude_enc_bit_ff Hcssrem) => Hencff.
     move : (enc_bits_copy (size r_rem) Hencff) => Henccpff.
-    move : (bit_blast_srem_correct Hbbsrem Hsz12 Hgt02 Henc1 Henc2 Hcssrem) => Hencr.
+    move : (bit_blast_srem_correct' Hbbsrem Hsz12 Hgt02 Henc1 Henc2 Hcssrem) => Hencr.
     move : (bit_blast_eq_correct Hbbeq2 Hszcprrem Hencr Henccpff Hcseq2).
-    rewrite (eqP Heq2) (add_prelude_enc_bit_true ((sremB bs1 bs2) == copy (size r_rem) false) Hcseq2). move => HsremB.
+    rewrite (eqP Heq2) (add_prelude_enc_bit_true ((sremB' bs1 bs2) == copy (size r_rem) false) Hcseq2). move => HsremB.
     rewrite (eqP HsremB) size_copy {1}/zeros {1}/b0 eq_refl orbT.
     rewrite (eqP HsremB) in Hencr. done.
   - case Heqf: (r_eq == lit_ff); case Heqf2: (r_eq2 == lit_ff).
     + rewrite/=; case => _ <- <-. move => Hsz12 Hgt02 Henc1 Henc2.
-      rewrite 3!add_prelude_catrev /smodB. move/andP => [Hcssrem Hcsu]; move/andP : Hcsu => [Hcseq Hcsu]; move/andP : Hcsu => [Hcseq2 Hcsadd].
+      rewrite 3!add_prelude_catrev /smodB'. move/andP => [Hcssrem Hcsu]; move/andP : Hcsu => [Hcseq Hcsu]; move/andP : Hcsu => [Hcseq2 Hcsadd].
       have Hszmsl12 : size [:: (splitmsl ls1).2] = size [:: (splitmsl ls2).2] by done.
       move : (add_prelude_tt Hcssrem) => Htt. move : (add_prelude_ff Hcssrem) => Hff. 
       move/andP : (enc_bits_splitmsb Htt Henc1) => [Henc1r Hencmsb1].
@@ -116,20 +110,20 @@ Proof.
       rewrite (add_prelude_enc_bit_is_not_true ([:: (splitmsb bs1).2] == [:: (splitmsb bs2).2]) Hcseq) Seqs.singleton_eq-/(msb bs1) -/(msb bs2).
       move/negP/eqP/eqP => Hmsb12. move : (Bool.not_true_is_false (msb bs1 == msb bs2) Hmsb12) => Hmsb12f.
       rewrite Hmsb12f orFb.
-      move : (bit_blast_srem_correct Hbbsrem Hsz12 Hgt02 Henc1 Henc2 Hcssrem) => Hencr.
+      move : (bit_blast_srem_correct' Hbbsrem Hsz12 Hgt02 Henc1 Henc2 Hcssrem) => Hencr.
       have Hszcprrem : size r_rem = size (copy (size r_rem) lit_ff) by rewrite size_nseq.
       move : (add_prelude_enc_bit_ff Hcssrem) => Hencff.
       move : (enc_bits_copy (size r_rem) Hencff) => Henccpff.
       move : (bit_blast_eq_correct Hbbeq2 Hszcprrem Hencr Henccpff Hcseq2).
-      rewrite (eqP Heqf2) (add_prelude_enc_bit_is_not_true ((sremB bs1 bs2) == copy (size r_rem) false) Hcseq2).
-      move/negP/eqP/eqP => HsremB. move : (Bool.not_true_is_false ((sremB bs1 bs2) == copy (size r_rem) false) HsremB) => HsremBnot0.
+      rewrite (eqP Heqf2) (add_prelude_enc_bit_is_not_true ((sremB' bs1 bs2) == copy (size r_rem) false) Hcseq2).
+      move/negP/eqP/eqP => HsremB. move : (Bool.not_true_is_false ((sremB' bs1 bs2) == copy (size r_rem) false) HsremB) => HsremBnot0.
       move : (enc_bits_size Hencr) => Hszencr.
       rewrite -Hszencr HsremBnot0.
-      generalize Hszencr. rewrite size_sremB -(enc_bits_size Henc1) Hsz12. move => Hszrrem.
-      move/eqP : (eq_refl (addB (sremB bs1 bs2) bs2)) => Haddr.
+      generalize Hszencr. rewrite size_sremB' -(enc_bits_size Henc1) Hsz12. move => Hszrrem.
+      move/eqP : (eq_refl (addB (sremB' bs1 bs2) bs2)) => Haddr.
       exact : (bit_blast_add_correct Hbbadd Hencr Henc2 Haddr Hcsadd Hszrrem).
     + rewrite/=. case => _ <- <-. move => Hsz12 Hgt02 Henc1 Henc2.
-      rewrite 6!add_prelude_catrev /smodB. move/andP => [Hcssrem Hcsu]; move/andP : Hcsu => [Hcseq Hcsu]; move/andP : Hcsu => [Hcseq2 Hcsu]; move/andP : Hcsu => [Hcsor Hcsu]; move/andP : Hcsu => [Hcsnot Hcsu]; move/andP : Hcsu => [Hcsand Hcsadd2].
+      rewrite 6!add_prelude_catrev /smodB'. move/andP => [Hcssrem Hcsu]; move/andP : Hcsu => [Hcseq Hcsu]; move/andP : Hcsu => [Hcseq2 Hcsu]; move/andP : Hcsu => [Hcsor Hcsu]; move/andP : Hcsu => [Hcsnot Hcsu]; move/andP : Hcsu => [Hcsand Hcsadd2].
       have Hszmsl12 : size [:: (splitmsl ls1).2] = size [:: (splitmsl ls2).2] by done.
       move : (add_prelude_tt Hcssrem) => Htt. move : (add_prelude_ff Hcssrem) => Hff. 
       move/andP : (enc_bits_splitmsb Htt Henc1) => [Henc1r Hencmsb1].
@@ -141,21 +135,21 @@ Proof.
       rewrite (add_prelude_enc_bit_is_not_true ([:: (splitmsb bs1).2] == [:: (splitmsb bs2).2]) Hcseq) Seqs.singleton_eq-/(msb bs1) -/(msb bs2).
       move/negP/eqP/eqP => Hmsb12. move : (Bool.not_true_is_false (msb bs1 == msb bs2) Hmsb12) => Hmsb12f.
       rewrite Hmsb12f orFb.
-      move : (bit_blast_srem_correct Hbbsrem Hsz12 Hgt02 Henc1 Henc2 Hcssrem) => Hencr.
+      move : (bit_blast_srem_correct' Hbbsrem Hsz12 Hgt02 Henc1 Henc2 Hcssrem) => Hencr.
       have Hszcprrem : size r_rem = size (copy (size r_rem) lit_ff) by rewrite size_nseq.
       move : (add_prelude_enc_bit_ff Hcssrem) => Hencff.
       move : (enc_bits_copy (size r_rem) Hencff) => Henccpff.
       move : (bit_blast_eq_correct Hbbeq2 Hszcprrem Hencr Henccpff Hcseq2) => Henceq2r.
-      case HsremB0: (sremB bs1 bs2 == zeros (size (sremB bs1 bs2))).
+      case HsremB0: (sremB' bs1 bs2 == zeros (size (sremB' bs1 bs2))).
       * move : (bit_blast_or_correct Hbbor (enc_bits_copy (size ls2) Henceqr) (enc_bits_copy (size ls2) Henceq2r) Hcsor).
-        rewrite -/(msb bs1) -/(msb bs2) Seqs.singleton_eq Hmsb12f (enc_bits_size Hencr) (eqP HsremB0) size_sremB size_zeros -/(zeros (size ls2)) eq_refl.
+        rewrite -/(msb bs1) -/(msb bs2) Seqs.singleton_eq Hmsb12f (enc_bits_size Hencr) (eqP HsremB0) size_sremB' size_zeros -/(zeros (size ls2)) eq_refl.
         have {1}-> : (size ls2 = size (copy (size ls2) true)) by rewrite size_nseq. rewrite or0B. 
         move => Hencorr.
         move : (bit_blast_not_correct Hbbnot Hencorr Hcsnot). rewrite invB_ones. move => Hencnotr.
         move : (bit_blast_and_correct Hbband2 Henc2 Hencnotr Hcsand). rewrite (enc_bits_size Henc2) andB0.
         move => Hencand2r.
-        have Haddr :(addB (zeros (size (sremB bs1 bs2))) (zeros (size bs2)) = zeros (size bs1)).
-        rewrite size_sremB add0B unzip2_zip; first by rewrite -(enc_bits_size Henc2) -Hsz12 (enc_bits_size Henc1).
+        have Haddr :(addB (zeros (size (sremB' bs1 bs2))) (zeros (size bs2)) = zeros (size bs1)).
+        rewrite size_sremB' add0B unzip2_zip; first by rewrite -(enc_bits_size Henc2) -Hsz12 (enc_bits_size Henc1).
         by rewrite 2!size_zeros -(enc_bits_size Henc2) -Hsz12 (enc_bits_size Henc1).
         rewrite -(eqP HsremB0) in Haddr.
         move : (bit_blast_srem_size_ss Hbbsrem) => Hszsrem.
@@ -170,14 +164,14 @@ Proof.
         move : (bit_blast_not_correct Hbbnot Hencorr Hcsnot). rewrite invB_zeros. move => Hencnotr.
         move : (bit_blast_and_correct Hbband2 Henc2 Hencnotr Hcsand). rewrite (enc_bits_size Henc2) andB1.
         move => Hencand2r.
-        move/eqP : (eq_refl (addB  (sremB bs1 bs2) bs2)) => Haddr.
+        move/eqP : (eq_refl (addB  (sremB' bs1 bs2) bs2)) => Haddr.
         move : (bit_blast_srem_size_ss Hbbsrem) => Hszsrem.
         move : (bit_blast_or_size_ss Hbbor) => Hszor. rewrite size_nseq in Hszor.
         move : (bit_blast_not_size_ss Hbbnot) => Hsznot. rewrite Hszor in Hsznot.
         move : (bit_blast_and_size_ss Hbband2 Hsznot) => Hszand2. rewrite -Hsz12 -Hszsrem in Hszand2.
         exact : (bit_blast_add_correct Hbbadd2 Hencr Hencand2r Haddr Hcsadd2 Hszand2).
     + rewrite /=. case => _ <- <-. move => Hsz12 Hgt02 Henc1 Henc2.
-      rewrite 6!add_prelude_catrev /smodB. move/andP => [Hcssrem Hcsu]; move/andP : Hcsu => [Hcseq Hcsu]; move/andP : Hcsu => [Hcseq2 Hcsu]; move/andP : Hcsu => [Hcsor Hcsu]; move/andP : Hcsu => [Hcsnot Hcsu]; move/andP : Hcsu => [Hcsand Hcsadd2].
+      rewrite 6!add_prelude_catrev /smodB'. move/andP => [Hcssrem Hcsu]; move/andP : Hcsu => [Hcseq Hcsu]; move/andP : Hcsu => [Hcseq2 Hcsu]; move/andP : Hcsu => [Hcsor Hcsu]; move/andP : Hcsu => [Hcsnot Hcsu]; move/andP : Hcsu => [Hcsand Hcsadd2].
       have Hszmsl12 : size [:: (splitmsl ls1).2] = size [:: (splitmsl ls2).2] by done.
       move : (add_prelude_tt Hcssrem) => Htt. move : (add_prelude_ff Hcssrem) => Hff. 
       move/andP : (enc_bits_splitmsb Htt Henc1) => [Henc1r Hencmsb1].
@@ -188,13 +182,13 @@ Proof.
       have Hszcprrem : size r_rem = size (copy (size r_rem) lit_ff) by rewrite size_nseq.
       move : (add_prelude_enc_bit_ff Hcssrem) => Hencff.
       move : (enc_bits_copy (size r_rem) Hencff) => Henccpff.
-      move : (bit_blast_srem_correct Hbbsrem Hsz12 Hgt02 Henc1 Henc2 Hcssrem) => Hencr.
+      move : (bit_blast_srem_correct' Hbbsrem Hsz12 Hgt02 Henc1 Henc2 Hcssrem) => Hencr.
       move : (bit_blast_eq_correct Hbbeq2 Hszcprrem Hencr Henccpff Hcseq2) => Henceq2r.
       generalize Henceq2r.
-      rewrite (eqP Heqf2) (add_prelude_enc_bit_is_not_true ((sremB bs1 bs2) == copy (size r_rem) false) Hcseq2). move => HsremB.
+      rewrite (eqP Heqf2) (add_prelude_enc_bit_is_not_true ((sremB' bs1 bs2) == copy (size r_rem) false) Hcseq2). move => HsremB.
       generalize HsremB.
-      move/negP/eqP/eqP => HsremB0. move : (Bool.not_true_is_false ((sremB bs1 bs2) == copy (size r_rem) false) HsremB0) => HsremB0f.
-      rewrite (enc_bits_size Hencr) -/(zeros (size (sremB bs1 bs2))) in HsremB0f.
+      move/negP/eqP/eqP => HsremB0. move : (Bool.not_true_is_false ((sremB' bs1 bs2) == copy (size r_rem) false) HsremB0) => HsremB0f.
+      rewrite (enc_bits_size Hencr) -/(zeros (size (sremB' bs1 bs2))) in HsremB0f.
       rewrite HsremB0f orbF.
       case Hmsbeq : (msb bs1 == msb bs2).
       * move : (bit_blast_or_correct Hbbor (enc_bits_copy (size ls2) Henceqr) (enc_bits_copy (size ls2) Henceq2r) Hcsor).
@@ -205,9 +199,9 @@ Proof.
         move : (bit_blast_not_correct Hbbnot Hencorr Hcsnot). rewrite invB_ones. move => Hencnotr.
         move : (bit_blast_and_correct Hbband2 Henc2 Hencnotr Hcsand). rewrite (enc_bits_size Henc2) andB0.
         move => Hencand2r.
-        have Haddr :(addB  (sremB bs1 bs2) (zeros (size bs2)) = (sremB bs1 bs2)).
+        have Haddr :(addB  (sremB' bs1 bs2) (zeros (size bs2)) = (sremB' bs1 bs2)).
         rewrite addB0 unzip1_zip; first done.
-        by rewrite size_sremB size_zeros -(enc_bits_size Henc2)-Hsz12 (enc_bits_size Henc1).
+        by rewrite size_sremB' size_zeros -(enc_bits_size Henc2)-Hsz12 (enc_bits_size Henc1).
         move : (bit_blast_srem_size_ss Hbbsrem) => Hszsrem.
         move : (bit_blast_or_size_ss Hbbor) => Hszor. rewrite size_nseq in Hszor.
         move : (bit_blast_not_size_ss Hbbnot) => Hsznot. rewrite Hszor in Hsznot.
@@ -221,14 +215,14 @@ Proof.
         move : (bit_blast_not_correct Hbbnot Hencorr Hcsnot). rewrite invB_zeros. move => Hencnotr.
         move : (bit_blast_and_correct Hbband2 Henc2 Hencnotr Hcsand). rewrite (enc_bits_size Henc2) andB1.
         move => Hencand2r.
-        move/eqP :(eq_refl (addB  (sremB bs1 bs2) bs2)) => Haddr.
+        move/eqP :(eq_refl (addB  (sremB' bs1 bs2) bs2)) => Haddr.
         move : (bit_blast_srem_size_ss Hbbsrem) => Hszsrem.
         move : (bit_blast_or_size_ss Hbbor) => Hszor. rewrite size_nseq in Hszor.
         move : (bit_blast_not_size_ss Hbbnot) => Hsznot. rewrite Hszor in Hsznot.
         move : (bit_blast_and_size_ss Hbband2 Hsznot) => Hszand2. rewrite -Hsz12 -Hszsrem in Hszand2.
         exact : (bit_blast_add_correct Hbbadd2 Hencr Hencand2r Haddr Hcsadd2 Hszand2).
     + rewrite /=. case => _ <- <-. move => Hsz12 Hgt02 Henc1 Henc2.
-      rewrite 6!add_prelude_catrev /smodB. move/andP => [Hcssrem Hcsu]; move/andP : Hcsu => [Hcseq Hcsu]; move/andP : Hcsu => [Hcseq2 Hcsu]; move/andP : Hcsu => [Hcsor Hcsu]; move/andP : Hcsu => [Hcsnot Hcsu]; move/andP : Hcsu => [Hcsand Hcsadd2].
+      rewrite 6!add_prelude_catrev /smodB'. move/andP => [Hcssrem Hcsu]; move/andP : Hcsu => [Hcseq Hcsu]; move/andP : Hcsu => [Hcseq2 Hcsu]; move/andP : Hcsu => [Hcsor Hcsu]; move/andP : Hcsu => [Hcsnot Hcsu]; move/andP : Hcsu => [Hcsand Hcsadd2].
       have Hszmsl12 : size [:: (splitmsl ls1).2] = size [:: (splitmsl ls2).2] by done.
       move : (add_prelude_tt Hcssrem) => Htt. move : (add_prelude_ff Hcssrem) => Hff. 
       move/andP : (enc_bits_splitmsb Htt Henc1) => [Henc1r Hencmsb1].
@@ -239,23 +233,23 @@ Proof.
       have Hszcprrem : size r_rem = size (copy (size r_rem) lit_ff) by rewrite size_nseq.
       move : (add_prelude_enc_bit_ff Hcssrem) => Hencff.
       move : (enc_bits_copy (size r_rem) Hencff) => Henccpff.
-      move : (bit_blast_srem_correct Hbbsrem Hsz12 Hgt02 Henc1 Henc2 Hcssrem) => [Hencr].
+      move : (bit_blast_srem_correct' Hbbsrem Hsz12 Hgt02 Henc1 Henc2 Hcssrem) => [Hencr].
       move : (bit_blast_eq_correct Hbbeq2 Hszcprrem Hencr Henccpff Hcseq2) => Henceq2r.
-      case Hmsbeq : (msb bs1 == msb bs2); last case Hmsbeq2 : ((sremB bs1 bs2) == zeros (size (sremB bs1 bs2))).
+      case Hmsbeq : (msb bs1 == msb bs2); last case Hmsbeq2 : ((sremB' bs1 bs2) == zeros (size (sremB' bs1 bs2))).
       * rewrite/=.
         have Hszcpeq : (size (copy (size ls2) r_eq)= size (copy (size ls2) r_eq2)) by rewrite 2!size_nseq.
         move : (bit_blast_or_correct Hbbor (enc_bits_copy (size ls2) Henceqr) (enc_bits_copy (size ls2) Henceq2r) Hcsor).
-        have {1}-> :(size ls2 = size (copy (size ls2) ((sremB bs1 bs2) == copy (size r_rem) false))) by rewrite size_nseq.
+        have {1}-> :(size ls2 = size (copy (size ls2) ((sremB' bs1 bs2) == copy (size r_rem) false))) by rewrite size_nseq.
         rewrite -/(msb bs1) -/(msb bs2) Seqs.singleton_eq Hmsbeq (enc_bits_size Hencr).
-        rewrite -/b1 -/(ones (size (copy (size ls2) ((sremB bs1 bs2) == copy (size (sremB bs1 bs2)) false)))) or1B size_nseq.
+        rewrite -/b1 -/(ones (size (copy (size ls2) ((sremB' bs1 bs2) == copy (size (sremB' bs1 bs2)) false)))) or1B size_nseq.
         move => Hencorr.
         move : (bit_blast_not_correct Hbbnot Hencorr Hcsnot). rewrite invB_ones. move => Hencnotr.
         move : (bit_blast_and_correct Hbband2 Henc2 Hencnotr Hcsand).
         rewrite (enc_bits_size Henc2) andB0.
         move => Hencand2r.
-        have Haddr :(addB  (sremB bs1 bs2) (zeros (size bs2)) = (sremB bs1 bs2)).
+        have Haddr :(addB  (sremB' bs1 bs2) (zeros (size bs2)) = (sremB' bs1 bs2)).
         rewrite addB0 unzip1_zip; first done.
-        by rewrite size_sremB -(enc_bits_size Henc2) -Hsz12 (enc_bits_size Henc1) size_zeros.
+        by rewrite size_sremB' -(enc_bits_size Henc2) -Hsz12 (enc_bits_size Henc1) size_zeros.
         move : (bit_blast_srem_size_ss Hbbsrem) => Hszsrem.
         move : (bit_blast_or_size_ss Hbbor) => Hszor. rewrite size_nseq in Hszor.
         move : (bit_blast_not_size_ss Hbbnot) => Hsznot. rewrite Hszor in Hsznot.
@@ -272,9 +266,9 @@ Proof.
         move : (bit_blast_not_correct Hbbnot Hencorr Hcsnot). rewrite invB_ones. move => Hencnotr.
         move : (bit_blast_and_correct Hbband2 Henc2 Hencnotr Hcsand). rewrite (enc_bits_size Henc2) andB0.
         move => Hencand2r.
-        have Haddr :(addB  (sremB bs1 bs2) (zeros (size bs2)) = (sremB bs1 bs2)).
+        have Haddr :(addB  (sremB' bs1 bs2) (zeros (size bs2)) = (sremB' bs1 bs2)).
         rewrite addB0 unzip1_zip; first done.
-        by rewrite size_sremB size_zeros -(enc_bits_size Henc2)-Hsz12 (enc_bits_size Henc1).
+        by rewrite size_sremB' size_zeros -(enc_bits_size Henc2)-Hsz12 (enc_bits_size Henc1).
         move : (bit_blast_srem_size_ss Hbbsrem) => Hszsrem.
         move : (bit_blast_or_size_ss Hbbor) => Hszor. rewrite size_nseq in Hszor.
         move : (bit_blast_not_size_ss Hbbnot) => Hsznot. rewrite Hszor in Hsznot.
@@ -290,7 +284,7 @@ Proof.
         move : (bit_blast_not_correct Hbbnot Hencorr Hcsnot). rewrite invB_zeros. move => Hencnotr.
         move : (bit_blast_and_correct Hbband2 Henc2 Hencnotr Hcsand). rewrite (enc_bits_size Henc2) andB1.
         move => Hencand2r.
-        have Haddr :(addB  (sremB bs1 bs2) bs2 = addB (sremB bs1 bs2) bs2) by done.
+        have Haddr :(addB  (sremB' bs1 bs2) bs2 = addB (sremB' bs1 bs2) bs2) by done.
         move : (bit_blast_srem_size_ss Hbbsrem) => Hszsrem.
         move : (bit_blast_or_size_ss Hbbor) => Hszor. rewrite size_nseq in Hszor.
         move : (bit_blast_not_size_ss Hbbnot) => Hsznot. rewrite Hszor in Hsznot.
@@ -298,6 +292,17 @@ Proof.
         exact : (bit_blast_add_correct Hbbadd2 Hencr Hencand2r Haddr Hcsadd2 Hszand2).
 Qed.
 
+Lemma bit_blast_smod_correct g ls1 ls2 g' cs rlrs E bs1 bs2 :
+  bit_blast_smod g ls1 ls2 = (g', cs, rlrs) ->
+  size ls1 = size ls2 ->
+  0 < size ls2 ->
+  enc_bits E ls1 bs1 ->
+  enc_bits E ls2 bs2 ->
+  interp_cnf E (add_prelude cs) ->
+  enc_bits E rlrs (smodB bs1 bs2).
+Proof.
+  rewrite smodB_is_smodB'. exact: bit_blast_smod_correct'.
+Qed.
 
 Definition mk_env_smod E g ls1 ls2 : env * generator * cnf * word :=
   let (ls1_tl, ls1_sign) := eta_expand (splitmsl ls1) in
